Clean up

src/graph_theory/cayley.lean
@@ -12,36 +12,34 @@ structure genset (G : Type*) [group G] :=
   (nem : els.nonempty)
   (irr : (1:G) ∉ els)
 
-variables {G : Type*} [group G] (S S1 S2 : genset G) (a : G) {x y z : G}
+variables {G : Type*} [group G] {S : genset G} (S1 S2 : genset G) (a : G) {x y z : G}
 
 instance : has_mem G (genset G) := ⟨λ a s, a ∈ s.els⟩
 
-def adj (x y : G) := x⁻¹ * y ∈ S
+def adj (S : genset G) (x y : G) := x⁻¹ * y ∈ S
 
-@[simp] lemma cancel (a x y : G) : (a * x)⁻¹ * (a * y) = x⁻¹ * y := by group
-
-lemma shift_adj {S : genset G} (h : adj S x y) : adj S (a*x) (a*y) :=
-by { unfold adj, rw cancel, exact h }
+lemma shift_adj (h : adj S x y) : adj S (a*x) (a*y) :=
+by { unfold adj, convert h using 1, group }
 
 @[symm] lemma adj_symm (x y) (h : adj S x y) : adj S y x
 := by { unfold adj, convert S.sym h, group }
 
 def Cay (S : genset G) : simple_graph G :=
 { adj := adj S,
-  symm := adj_symm S,
+  symm := adj_symm,
   loopless := λ x h, S.irr (by { convert h, group }) }
 
 def left_shift : (Cay S) →g (Cay S) :=
 ⟨(*) a, λ x y, shift_adj a⟩
 
 def shift_path (p : walk (Cay S) x y) : walk (Cay S) (a*x) (a*y) :=
-p.map (left_shift S a)
+p.map (left_shift a)
 
 lemma shift : reachable (Cay S) x y → reachable (Cay S) (a*x) (a*y) :=
-nonempty.map (shift_path S a)
+nonempty.map (shift_path a)
 
 lemma inv : reachable (Cay S) 1 x → reachable (Cay S) 1 x⁻¹ :=
-by { intro h, symmetry, convert shift S x⁻¹ h; group }
+by { intro h, symmetry, convert shift x⁻¹ h; group }
 
 lemma reachable_mp : reachable (Cay S) 1 x :=
 begin
@@ -49,11 +47,11 @@ begin
   { rw S.gen, trivial },
   { intros y h, apply reachable.step, simp only [Cay,adj], convert h, group },
   { refl },
-  { intros u v h1 h2, refine reachable.trans h1 _, convert shift _ u h2, group },
+  { intros u v h1 h2, refine reachable.trans h1 _, convert shift u h2, group },
   { intros y h, apply inv, exact h }
 end
 
-theorem connected : connected (Cay S) :=
+theorem connected (S : genset G) : connected (Cay S) :=
 begin
   split,
   { intros x y, transitivity (1:G), symmetry, apply reachable_mp, apply reachable_mp },
@@ -67,11 +65,11 @@ set.range (length : walk G x y -> ℕ)
 lemma covariant' : (Cay S).dist (a*x) (a*y) ≤ (Cay S).dist x y :=
 begin
   obtain ⟨p,hp⟩ := (connected S).exists_walk_of_dist x y, rw ←hp, clear hp,
-  rw ←walk.length_map, exact dist_le (shift_path S a p)
+  rw ←walk.length_map, exact dist_le (shift_path a p)
 end
 
 lemma covariant : (Cay S).dist (a*x) (a*y) = (Cay S).dist x y :=
-by { apply le_antisymm (covariant' S a), convert covariant' S a⁻¹; group }
+by { apply le_antisymm (covariant' a), convert covariant' a⁻¹; group }
 
 noncomputable def distorsion (S1 S2 : genset G) :=
 some (max_of_nonempty (S1.nem.image ((Cay S2).dist 1)))
@@ -82,7 +80,7 @@ some_spec (max_of_nonempty (S1.nem.image ((Cay S2).dist 1)))
 lemma distorsion_le {h : (Cay S1).adj x y} : (Cay S2).dist x y ≤ distorsion S1 S2 :=
 begin
   refine finset.le_max_of_mem _ (distorsion_spec S1 S2),
-  rw [finset.mem_image], refine ⟨x⁻¹ * y, h, _⟩, convert covariant _ x⁻¹, group
+  rw [finset.mem_image], refine ⟨x⁻¹ * y, h, _⟩, convert covariant x⁻¹, group
 end
 
 lemma lipschitz : (Cay S2).dist x y <= (distorsion S1 S2) * (Cay S1).dist x y :=
